apc/APC.v
@@ -73,7 +73,7 @@ Section apc.
 End apc.
 
 Section aux.
-  Context `{_crisG: !crisG  Γ Σ α β τ _S _I _T}.
+  Context `{_crisG: !crisG Γ Σ α β τ _S _I}.
 
   Lemma map_fst_map_map_snd_refl {A B C} (f: B → C) (l: list (A * B)):
     map fst (map (map_snd f) l) = map fst l.
