theories/cancellation/Cancel.v
@@ -1,0 +1,153 @@
+Require Import Common.
+From iris.proofmode Require Import proofmode.
+Require Import SModTr HModTr ModTr SMod HMod Mod.
+Require Import ITactics TacticsCommon SimGlobal SimGlobalFacts CtxRefine ClosedAdequacy.
+Require Import HModInline HModInlineIntro HModInlineElim ElimRel.
+Require Import SimGlobal SimGTactics.
+Require Import CancelSpawn CancelCore CancelPG CancelAG CancelPre CancelPost.
+
+Set Implicit Arguments.
+
+Module Cancel. Section Cancel.
+
+Context `{Σ: GRA}.
+
+Lemma cancel_elim md sp (rs0 r_s r_t: Σ) srcs tgts cid st ps pt
+  (WFS: smod_wf md)
+  (VP: valid_sp md sp)
+  (WF: HMod.wf (SMod.to_hmod sp_none (SMod.cancel md)))
+  (REL: Forall2i (thread_rel sp) srcs tgts)
+  (WFR: ✓ r_s)
+  (RS: Own r_s ⊢ |==> Own r_t)
+  :
+  simg cancel_eq ps pt
+    (ModTr.interp_stateE Any.t
+       (iterV (ModTr.handle_callE (Mod.prog (HMod.to_mod (HModInline.inline
+              (SMod.to_hmod sp_none (SMod.cancel md))) rs0))) (cid, srcs))
+       (Any.pair (HModTr.alist_encode st) r_s ↑))
+    (ModTr.interp_stateE Any.t
+       (iterV (ModTr.handle_callE (Mod.prog (HMod.to_mod (HModInline.inline
+              (SMod.to_hmod sp md)) rs0))) (cid, tgts))
+       (Any.pair (HModTr.alist_encode st) r_t ↑)).
+Proof.
+  ginit. move WFS at top. move WF at top. move VP at top.
+  revert_until rs0. gcofix CIH. i.
+  destruct (classic (cid < length srcs)); cycle 1.
+  { ziter_l. erewrite (proj2 (lookup_ge_None srcs cid)); try nia.
+    s. zstep_l. zstep_l. }
+  rename H into LEN. exploit Forall2i_nth; eauto. i. des. ss.
+  rename x into src, y into tgt. depdes x2.
+  destruct REL as [EQLEN REL].
+
+  assert(KEY: ∀ itrS' itrT' st (r_s r_t: Σ) tid
+                 (WFR: ✓ r_s)
+                 (RS: Own r_s ⊢ |==> Own r_t)
+                 (LEN: cid < List.length srcs)
+                 (REL: elim_rel sp itrS' itrT'),
+  gpaco7 _simg (cpn7 _simg) bot7 r (Any.t * Any.t)%type
+    (Any.t * Any.t)%type cancel_eq smj_top smj_top
+    (ModTr.interp_stateE Any.t
+       (iterV (ModTr.handle_callE (Mod.prog (HMod.to_mod (HModInline.inline
+              (SMod.to_hmod sp_none (SMod.cancel md))) rs0)))
+              (tid, <[cid:=interpV HModTr.handle_hmodE itrS']> srcs))
+       (Any.pair (HModTr.alist_encode st) r_s ↑))
+    (ModTr.interp_stateE Any.t
+       (iterV (ModTr.handle_callE (Mod.prog (HMod.to_mod (HModInline.inline
+              (SMod.to_hmod sp md)) rs0)))
+              (tid, <[cid:=x_ <- interpV HModTr.handle_hmodE itrT';; k x_]> tgts))
+       (Any.pair (HModTr.alist_encode st) r_t ↑))).
+  {
+    i. zprogress.
+    gbase. eapply CIH; et.
+    econs. { rewrite !length_insert. et. }
+    i. destruct (classic (cid = i)); cycle 1.
+    { rewrite list_lookup_insert_ne in EQx; et.
+      rewrite list_lookup_insert_ne in EQy; et. }
+    subst. rewrite !list_lookup_insert in EQx, EQy; et; cycle 1.
+    { rewrite -EQLEN. et. }
+    inv EQx. econs; et.
+  }
+
+  punfold REL0. depdes REL0; ii; subst; pclearbot.
+  - ziter_r. rewrite x1. s. zstep_r.
+  - ziter_l. rewrite x0. s. zstep_l.
+  - ziter_l. rewrite x0. s. zstep_l. ziter_l. zstep_l.
+  - ziter_l. ziter_r. rewrite x0 x1. s. destruct cid; s; cycle 1.
+    { zstep_l. zstep_l. }
+    specialize (RET eq_refl). subst. s. zstep_l. zstep_r.
+    gstep. econs. econs.
+    r. esplits; et; hss.
+  - ziter_l. ziter_r. rewrite x0 x1. s. zstep_l. zstep_r. eapply KEY; et.
+  - eapply cancel_core; et.
+  - eapply cancel_pg; et.
+  - eapply cancel_ag; et.
+  - ziter_l. ziter_r. rewrite x0 x1. s. zstep_l. zstep_r. eapply KEY, KTR; et.
+  - eapply cancel_spawn; et.
+  - eapply cancel_pre; et.
+  - eapply cancel_post; et.
+Unshelve. all: try exact smj_top.
+(*SLOW*)Qed.
+
+Lemma cancel_main md sp rs
+  (WFS: smod_wf md)
+  (VP: valid_sp md sp)
+  (WF: HMod.wf (SMod.to_hmod sp_none (SMod.cancel md)))
+  (VALID: ✓ rs)
+  :  
+  refines_mod
+    (HMod.to_mod (HModInline.inline (SMod.to_hmod sp_none (SMod.cancel md))) rs)
+    (HMod.to_mod (HModInline.inline (SMod.to_hmod sp md)) rs).
+Proof.
+  r. intro arg. eapply adequacy_global.
+  instantiate (1:= smj_top). instantiate (1:= smj_top).
+  unfold Mod.compile. s. rewrite /ITree.map /ModTr.trans /ModTr.interp_callE.  
+
+  rewrite !alist_find_map_snd.
+  destruct (alist_find None (SMod.fnsems md)) eqn: FIND; rewrite FIND; cycle 1.
+  { s. ired. ginit. gstep. econs. econs. ss. }
+  s. ired. rewrite /HModTr.trans_ktree.
+  destruct f as [[[img msk] scp] [fspo bd]]. s.
+  assert (SCP: incl scp (SMod.scopes md)).
+  { ii. eapply SMod.well_scoped_fns. rewrite /fnsems_scopes. erewrite FIND. et. }
+  erewrite sandbox_inline_commute; et.
+  erewrite sandbox_inline_commute; et.
+  rewrite /SB.sandbox_body. s.
+
+  ginit. guclo bindC_spec. econs; cycle 1.
+  { instantiate (1:=cancel_eq). i. gstep. econs. econs.
+    destruct SIM. des. et. }
+  gfinal. right.
+
+  eapply cancel_elim; et. econs; et.
+  i. destruct i; ss. inv EQx.
+  exploit WFS; et. i. subst.
+  rewrite !if_prod_comm !if_simpl.
+  econs; et; cycle 1.
+  { rewrite bind_ret_r. et. }
+
+  s. eapply elim_rel_cancel; try r; et.
+Unshelve. all: exact smj_top.
+(*SLOW*)Qed.
+
+(*** Final Theorem ***)
+Theorem cancellation md sp P
+  (WFS: smod_wf md)
+  (VP: valid_sp md sp)
+  (WF: HMod.wf (SMod.to_hmod sp_none (SMod.cancel md)))
+  :
+  refines (SMod.to_hmod sp_none (SMod.cancel md), P)
+          (SMod.to_hmod sp md, P).
+Proof. 
+  etrans.
+  { eapply inline_elim. }
+  etrans; cycle 1.
+  { eapply inline_intro. }
+  ii; split.
+  {
+    inv WFM. econs; eauto. s.
+    repeat rewrite List.map_map fst_map_snd.
+    repeat rewrite List.map_map fst_map_snd in wf_fns. eauto.
+  }
+  inv WFM. s; i. exists rs. esplits; et.
+  eapply cancel_main; eauto.
+(*SLOW*)Qed.
