theories/cancellation/CancelAG.v
@@ -1,0 +1,38 @@
+Require Import Common.
+From iris.proofmode Require Import proofmode.
+Require Import SModTr HModTr ModTr SMod HMod Mod.
+Require Import ITactics TacticsCommon SimGlobal SimGlobalFacts CtxRefine ClosedAdequacy.
+Require Import HModInline HModInlineIntro HModInlineElim ElimRel.
+Require Import SimGlobal SimGTactics.
+
+Lemma cancel_ag `{Σ: GRA} md sp R (e : agE R):
+  CANCEL_GOAL md sp (trigger e) (trigger e).
+Proof.
+  r; i. destruct e.
+  + ziter_l. ziter_r. rewrite x0 x1. s. zstep_l. zstep_r. ss. ired. hss. ired.
+    ziter_l. do 2 zstep_l. ziter_r. zstep_r. eexists. zstep_r.
+    ziter_l. do 2 zstep_l. ziter_r. zstep_r. eexists. zstep_r.
+    ziter_l. zstep_l. ziter_r. zstep_r.
+    ziter_l. zstep_l. ziter_r. zstep_r.
+    des. eapply KEY, KTR; et.
+  + ziter_l. ziter_r. rewrite x0 x1. s. zstep_l. zstep_r. ss. ired. hss. ired.
+    ziter_r. do 2 zstep_r. ziter_l. zstep_l. eexists. zstep_l.
+    ziter_r. do 2 zstep_r. ziter_l. zstep_l. eexists. zstep_l.
+    ziter_r. do 2 zstep_r. ziter_l. zstep_l. eexists. zstep_l.
+    ziter_l. do 2 zstep_l. ziter_r. zstep_r. eexists. zstep_r.
+    ziter_l. zstep_l. ziter_r. zstep_r.
+    ziter_l. zstep_l. ziter_r. zstep_r.
+    des. eapply KEY, KTR; et.
+  + ziter_l. ziter_r. rewrite x0 x1. s. zstep_l. zstep_r. ss. ired. hss. ired.
+    ziter_r. do 2 zstep_r. ziter_l. zstep_l. eexists. zstep_l.
+    ziter_r. do 2 zstep_r. ziter_l. zstep_l. eexists. zstep_l.
+    ziter_l. zstep_l. ziter_r. zstep_r.
+    ziter_l. zstep_l. ziter_r. zstep_r.
+    des. eapply KEY, KTR; et.
+Unshelve. all: et; try exact smj_top.
+- des; et. split; et. rewrite RS in x3.
+  iIntros "H". iMod (x3 with "H") as "[P O]". iFrame. et.
+- rewrite RS. iIntros ">H". iApply x3. et.
+- des; et. split; et. rewrite RS.
+  iIntros ">H". iApply x3. et.
+(*SLOW*)Qed.
