theories/cancellation/CancelCore.v
@@ -1,52 +1,19 @@
 Require Import Common.
 From iris.proofmode Require Import proofmode.
 Require Import SModTr HModTr ModTr SMod HMod Mod.
+Require Import ITactics TacticsCommon SimGlobal SimGlobalFacts CtxRefine ClosedAdequacy.
+Require Import HModInline HModInlineIntro HModInlineElim ElimRel.
 Require Import SimGlobal SimGTactics.
-Require Import SModCancel HModInline ElimRel CancelLib.
 
-Lemma cancel_aux_core `{Σ: GRA} md
-  r ps pt srcs tgts cid st (rs rt rs0 rt0: Σ) l X (meta: X) Q R ktrS ktrT
-  (WFS: ✓ rs) (WFT: ✓ rt)
-  (UPD: Own rs ==∗ Own rt)
-  (LENS: cid < List.length srcs)
-  (LENT: cid < List.length tgts)
-  (LEN: List.length srcs = Datatypes.length tgts)
-  (RET: ∀ vret ret : Any.t, cid = 0 → Q meta vret ret ⊢ ⌜vret = ret⌝)
-  (RELS: ∀ k x y, cid ≠ k → srcs !! k = Some x → tgts !! k = Some y → thread_rel md k x y)
-  (KTR: ∀ x, paco3 (@elim_rel_def _ md _) bot3 l (ktrS x) (ktrT x))
-  (CIH: ∀ rs rt srcs tgts cid st ps pt X (meta : X) Q itrS itrT l,
-      ✓ rs → (Own rs ==∗ Own rt) →
-      List.length srcs = List.length tgts →
-      cid < List.length srcs → cid < List.length tgts → 
-      srcs !! cid = Some (HModTr.trans itrS) →
-      tgts !! cid = Some (HModTr.trans (cancel_term md meta Q itrT)) →
-      (∀ vret ret, cid = 0 → Q meta vret ret ⊢ ⌜vret = ret⌝) →
-      paco3 (@elim_rel_def _ md _) bot3 l itrS itrT →
-      (∀ k x y, cid ≠ k → srcs !! k = Some x → tgts !! k = Some y → thread_rel md k x y)
-      → CANCEL_GOAL md r rs0 rt0 ps pt srcs tgts cid st rs rt)
-
-  (e: coreE R)
-  (SRC : srcs !! cid = Some (HModTr.trans (x <- trigger e;; ktrS x)))
-  (TGT : tgts !! cid = Some (HModTr.trans (cancel_term md meta Q (x <- trigger e;; ktrT x))))
-  :
-  CANCEL_GOAL md (gpaco7 _simg (cpn7 _simg) bot7 r) rs0 rt0 ps pt srcs tgts cid st rs rt.
+Lemma cancel_core `{Σ: GRA} md sp R (e : coreE R):
+  CANCEL_GOAL md sp (trigger e) (trigger e).
 Proof.
-  r.
-  ziter_l. ziter_r. rewrite SRC TGT.
-  depdes e.
-  + zstep_r. zstep_r.
-    zstep_l. exists x. zstep_l.
-    zprogress.
-    gbase. eapply CIH; zsimpl_len; try zlookup_insert; et.
-    intros ? ? ? ?. do 2 zlookup_insert_ne. eauto.
-  + zstep_l. zstep_l.
-    zstep_r. exists x. zstep_r.
-    zprogress.
-    gbase. eapply CIH; zsimpl_len; try zlookup_insert; et.
-    intros ? ? ? ?. do 2 zlookup_insert_ne. eauto.
-  + zstep. zstep_l. zstep_r. subst.
-    zprogress.
-    gbase. eapply CIH; zsimpl_len; try zlookup_insert; et.
-    intros ? ? ? ?. do 2 zlookup_insert_ne. eauto.
-Unshelve. all: eauto.
+  r; i. destruct e.
+  + ziter_l. ziter_r. rewrite x0 x1. s. do 2 zstep_r. zstep_l. eexists. zstep_l.
+    eapply KEY, KTR; et.
+  + ziter_l. ziter_r. rewrite x0 x1. s. do 2 zstep_l. zstep_r. eexists. zstep_r.
+    eapply KEY, KTR; et.
+  + ziter_l. ziter_r. rewrite x0 x1. s. zstep. zstep_l. zstep_r. subst.
+    eapply KEY, KTR; et.
+Unshelve. all: exact smj_top.
 (*SLOW*)Qed.
