theories/cancellation/CancelPost.v
@@ -1,0 +1,118 @@
+Require Import Common.
+From iris.proofmode Require Import proofmode.
+Require Import SModTr HModTr ModTr SMod HMod Mod.
+Require Import ITactics TacticsCommon SimGlobal SimGlobalFacts CtxRefine ClosedAdequacy.
+Require Import HModInline HModInlineIntro HModInlineElim ElimRel.
+Require Import SimGlobal SimGTactics.
+
+Lemma cancel_post `{Σ: GRA} md sp:
+  ∀ (rs0: Σ) r_s r_t srcs tgts cid st ps pt vret X X' x x' Qo Qo' itrS ktrT k
+    (r: ∀ x x0, (x→x0→Prop)→smj→smj→itree coreE x→itree coreE x0→Prop)
+    (WFS: smod_wf md)
+    (VP: valid_sp md sp)
+    (WF: HMod.wf (SMod.to_hmod sp_none (SMod.cancel md)))
+    (KEY: ∀ itrS' itrT' st (r_s r_t: Σ) tid
+             (WFR: ✓ r_s)
+             (RS: Own r_s ⊢ |==> Own r_t)
+             (LEN: cid < List.length srcs)
+             (REL: elim_rel sp itrS' itrT'),
+     gpaco7 _simg (cpn7 _simg) bot7 r (Any.t * Any.t)%type
+       (Any.t * Any.t)%type cancel_eq smj_top smj_top
+       (ModTr.interp_stateE Any.t
+          (iterV (ModTr.handle_callE (Mod.prog (HMod.to_mod (HModInline.inline
+                 (SMod.to_hmod sp_none (SMod.cancel md))) rs0)))
+                 (tid, <[cid:=interpV HModTr.handle_hmodE itrS']> srcs))
+          (Any.pair (HModTr.alist_encode st) r_s ↑))
+       (ModTr.interp_stateE Any.t
+          (iterV (ModTr.handle_callE (Mod.prog (HMod.to_mod (HModInline.inline
+                 (SMod.to_hmod sp md)) rs0)))
+                 (tid, <[cid:=x_ <- interpV HModTr.handle_hmodE itrT';; k x_]> tgts))
+          (Any.pair (HModTr.alist_encode st) r_t ↑)))
+    (EQLEN : length srcs = length tgts)
+    (REL : ∀ i x y, srcs !! i = Some x → tgts !! i = Some y → thread_rel sp i x y)
+    (WFR : ✓ r_s)
+    (RS : Own r_s ⊢ |==> Own r_t)
+    (LEN : cid < length srcs)
+    (x0 : srcs !! cid = Some (HModTr.trans (tau;; tau;; itrS)))
+    (x1 : tgts !! cid = Some (x <- HModTr.trans (x <- elim_postcond Qo Qo' x x' vret;; ktrT x);; k x))
+    (RET : cid = 0 → k = λ x : Any.t, Ret x)
+    (KTR :
+    ∃ Q : X → Any.t → Any.t → iProp Σ,
+      (Qo = Some Q
+       ∨ Qo = None ∧ Q = λ (_ : X) (varg arg : Any.t), ⌜varg = arg⌝%I)
+      ∧ ∃ Q' : X' → Any.t → Any.t → iProp Σ,
+          (Qo' = Some Q'
+           ∨ Qo' = None ∧ Q' = λ (_ : X') (varg arg : Any.t), ⌜varg = arg⌝%I)
+          ∧ (∀ ret : Any.t, Q' x' vret ret ⊢ |==> Q x vret ret)
+            ∧ upaco3 (elim_rel_def sp) bot3 Any.t itrS (ktrT vret)),
+
+  gpaco7 _simg (cpn7 _simg) bot7 r (Any.t * Any.t)%type 
+    (Any.t * Any.t)%type cancel_eq ps pt
+    (ModTr.interp_stateE Any.t
+       (iterV (ModTr.handle_callE (Mod.prog (HMod.to_mod (HModInline.inline
+              (SMod.to_hmod sp_none (SMod.cancel md))) rs0))) (cid, srcs))
+       (Any.pair (HModTr.alist_encode st) r_s ↑))
+    (ModTr.interp_stateE Any.t
+       (iterV (ModTr.handle_callE (Mod.prog (HMod.to_mod (HModInline.inline
+              (SMod.to_hmod sp md)) rs0))) (cid, tgts))
+       (Any.pair (HModTr.alist_encode st) r_t ↑)).
+Proof.
+  i. ziter_l. ziter_r. rewrite x0 x1. s. zstep_l. ziter_l. zstep_l.
+  move KTR at bottom. des_safe.
+  destruct KTR0; subst; des_safe.
+  {
+    zstep_r. zstep_r.
+    ziter_r. zstep_r. ziter_r. zstep_r.
+    ziter_r. zstep_r. zstep_r. ziter_r. zstep_r. zstep_r.
+    ziter_r. zstep_r. ziter_r. zstep_r. ziter_r. zstep_r.
+    ziter_r. zstep_r. ziter_r. zstep_r.
+
+    des; subst.
+    {
+      ziter_r. zstep_r. eexists. zstep_r.
+      ziter_r. zstep_r. ziter_r. zstep_r.
+      ziter_r. zstep_r. eexists r_t. zstep_r.
+      ziter_r. zstep_r. unshelve eexists.
+      { split; eauto using Own_wand_valid.
+        iIntros "H". iMod (x5 with "H") as "[P O]". rewrite KTR1. iFrame. 
+      }
+      zstep_r.
+      ziter_r. zstep_r. ziter_r. zstep_r. ziter_r. zstep_r.
+
+      pclearbot. eapply KEY; et.
+    }
+    {
+      assert (vret = x2).
+      { eapply Own_pure_soundness; try apply WFR.
+        rewrite RS. iIntros ">H". iMod (x5 with "H") as "[P O]".
+        rewrite KTR1. iMod "P" as "P"; et.
+      }
+      des. subst.
+      ired. pclearbot. eapply KEY; et.
+      rewrite RS. iIntros ">H". iMod (x5 with "H") as "[P O]". iFrame. et.
+    }
+  }
+  {
+    s. zstep_r.
+    des; subst.      
+    {
+      ziter_r. zstep_r.
+      ziter_r. zstep_r. eexists. zstep_r.
+      ziter_r. zstep_r. ziter_r. zstep_r.
+      ziter_r. zstep_r. eexists r_t. zstep_r.
+      ziter_r. zstep_r. unshelve eexists.
+      { split; eauto using Own_wand_valid.
+        iIntros "H". iFrame. iApply KTR1. et.
+      }
+      zstep_r.
+      ziter_r. zstep_r. ziter_r. zstep_r. ziter_r. zstep_r.
+
+      pclearbot. eapply KEY; et.
+    }
+    {
+      ziter_r. zstep_r.
+      pclearbot. eapply KEY; et.
+    }
+  }
+Unshelve. all: try exact smj_top.
+(*SLOW*)Qed.
